Support guarded pDOT: Allow paths as value definitions
Most crucially, define path_wp as a least fixpoint.

The new API is enough for the remaining code, as shown by
https://github.com/Blaisorblade/dot-iris/pull/153.

theories/Dot/lr/path_wp.v
@@ -19,18 +19,33 @@ Proof. by elim: p => [v| p /= ->]. Qed.
 Lemma path2tm_subst p ρ: (path2tm p).|[ρ] = path2tm p.|[ρ].
 Proof. by elim: p => /= [//|p -> l]. Qed.
 
-(** * Pure path weakest precondition. *)
-Fixpoint path_wp_pure p Pv : Prop :=
-  match p with
-  | pself p l => path_wp_pure p (λ v, ∃ w, v @ l ↘ dvl w ∧ Pv w)
-  | pv vp => Pv vp
-  end.
+(** A simplified variant of weakest preconditions for path evaluation.
+The difference is that path evaluation is completely pure, and
+postconditions must hold now, not after updating resources.
+vp ("Value from Path") and vq range over results of evaluating paths.
+Below, we define a version internal to Iris, following Iris's total weakest
+precondition. *)
+
+Inductive path_wp_pure : path → (vl → Prop) → Prop :=
+| pwp_pv vp Pv : Pv vp → path_wp_pure (pv vp) Pv
+| pwp_pself p vp q l Pv : path_wp_pure p (eq vp) → vp @ l ↘ dvl q → path_wp_pure q Pv →
+  path_wp_pure (pself p l) Pv .
+Local Hint Constructors path_wp_pure : core.
+
+Lemma path_wp_pure_inv_pv Pv v : path_wp_pure (pv v) Pv ↔ Pv v.
+Proof. split; by [inversion_clear 1 | auto]. Qed.
+
+Lemma path_wp_pure_inv_pself Pv p l : path_wp_pure (pself p l) Pv →
+  ∃ vp q, path_wp_pure p (eq vp) ∧ vp @ l ↘ dvl q ∧ path_wp_pure q Pv ∧
+  path_wp_pure (pself p l) Pv.
+Proof. inversion_clear 1; naive_solver. Qed.
 
 Global Instance Proper_pwp_pure: Proper ((=) ==> pointwise_relation _ iff ==> iff) path_wp_pure.
 Proof.
   (* The induction works best in this shape, but this instance is best kept local. *)
   have Proper_pwp_2: ∀ p, Proper (pointwise_relation _ iff ==> iff) (path_wp_pure p).
-  elim; solve_proper.
+  by rewrite /pointwise_relation => p P1 P2 HPeq; split;
+    induction 1; naive_solver.
   solve_proper.
 Qed.
 
@@ -38,24 +53,14 @@ Lemma path_wp_pure_wand {Pv1 Pv2 p}:
   path_wp_pure p Pv1 →
   (∀ v, Pv1 v → Pv2 v) →
   path_wp_pure p Pv2.
-Proof.
-  elim: p Pv1 Pv2 => /= [v|p IHp l] Pv1 Pv2 Hp Hwand;
-    first by apply Hwand.
-  apply: (IHp _ _ Hp) => {IHp Hp} v [vq [??]].
-  eauto.
-Qed.
+Proof. elim; eauto. Qed.
 
 Lemma path_wp_pure_eq p Pv :
   path_wp_pure p Pv ↔ ∃ v, path_wp_pure p (eq v) ∧ Pv v.
 Proof.
-  elim: p Pv => [ v | p IHp l ] Pv /=; split.
-  - eauto.
-  - by destruct 1 as (w & <- & ?).
-  - rewrite IHp; intros (v & Hp & w & ?&?).
-    eexists w; split; last by [].
-    apply (path_wp_pure_wand Hp).
-    intros v' ->; exists w; eauto.
-  - setoid_rewrite IHp; intros; ev; subst; eauto.
+  split.
+  - elim; naive_solver.
+  - move => [v [Hpeq HPv]]. dependent induction Hpeq; naive_solver.
 Qed.
 
 Lemma path_wp_pure_det {p v1 v2}:
@@ -63,10 +68,12 @@ Lemma path_wp_pure_det {p v1 v2}:
   path_wp_pure p (eq v2) →
   v1 = v2.
 Proof.
-  elim: p v1 v2 => [v /=| p /= IHp l //] v1 v2; first by intros <- <-.
-  rewrite !path_wp_pure_eq; intros (w1 & Hp1 & ?) (w2 & Hp2 & ?);
-    move: (IHp _ _ Hp1 Hp2) => ?; ev; simplify_eq.
-  by objLookupDet.
+  move => Hp1 Hp2; move: v2 Hp2; induction Hp1; intros; inverse Hp2; first naive_solver.
+  lazymatch goal with H1 : ?vp @ l ↘ dvl ?q, H2 : ?vp0 @ l ↘ dvl ?q0 |- _ =>
+    (suff ?: q = q0 by subst; auto);
+    (suff ?: vp = vp0 by subst; objLookupDet);
+    auto
+  end.
 Qed.
 
 Lemma path_wp_pure_swap p w :
@@ -78,14 +85,14 @@ Lemma path_wp_exec_pure p v :
   path_wp_pure p (eq v) →
   ∃ n, PureExec True n (path2tm p) (tv v).
 Proof.
-  elim: p v => [w|p IHp l] v; rewrite /PureExec/=.
-  by intros ->; eexists; constructor.
-  rewrite path_wp_pure_eq; intros (vp & Hp & vq & Hlook & ->).
-  move: (IHp _ Hp) => [n Hpure].
-  exists (S n) => _.
-  eapply nsteps_r.
-  - by apply (pure_step_nsteps_ctx (fill_item (ProjCtx l))), Hpure.
-  - apply nsteps_once_inv, pure_tproj, Hlook.
+  move HE: (eq v) => P Hp; move: v HE; induction Hp; intros; simplify_eq.
+  by exists 0; constructor.
+  have [m /(_ I) Hs1] := IHHp1 _ eq_refl.
+  have [n /(_ I) Hs2] := IHHp2 _ eq_refl.
+  exists (S m + n) => _ /=.
+  eapply (nsteps_trans (S m)), Hs2; eapply nsteps_r.
+  by apply (pure_step_nsteps_ctx (fill_item (ProjCtx l))), Hs1.
+  by apply nsteps_once_inv, pure_tproj.
 Qed.
 
 Definition alias_paths p q :=
@@ -93,13 +100,16 @@ Definition alias_paths p q :=
 
 Lemma alias_paths_pv_eq_1 p vr :
   alias_paths p (pv vr) ↔ path_wp_pure p (eq vr).
-Proof. done. Qed.
+Proof. rewrite /alias_paths. by setoid_rewrite path_wp_pure_inv_pv. Qed.
 
 Hint Extern 1 (path_wp_pure _ _) => by apply path_wp_pure_swap : core.
 
 Lemma alias_paths_pv_eq_2 p vr :
   alias_paths (pv vr) p ↔ path_wp_pure p (eq vr).
-Proof. by rewrite -path_wp_pure_swap. Qed.
+Proof.
+  rewrite /alias_paths -path_wp_pure_swap.
+  by setoid_rewrite path_wp_pure_inv_pv.
+Qed.
 
 Lemma alias_paths_self p v :
   alias_paths p (pv v) → alias_paths p p.
@@ -109,7 +119,7 @@ Qed.
 
 Lemma alias_paths_refl_vl v :
   alias_paths (pv v) (pv v).
-Proof. done. Qed.
+Proof. hnf; eauto. Qed.
 
 Lemma alias_paths_sameres p q:
   alias_paths p q ↔
@@ -153,48 +163,160 @@ Lemma alias_paths_elim_eq_pure Pv {p q}:
   path_wp_pure p Pv ↔ path_wp_pure q Pv.
 Proof. move => /alias_paths_samepwp_pure [_]. apply. Qed.
 
-Section path_wp.
+From iris.bi Require Import fixpoint big_op.
+(* From iris.program_logic Require Export weakestpre. *)
+Set Default Proof Using "Type".
+Import uPred.
+
+Canonical Structure pathO := leibnizO path.
+Canonical Structure vlO := leibnizO vl.
+
+Section path_wp_pre.
   Context {Σ : gFunctors}.
   Implicit Types (φ : vl -d> iPropO Σ).
 
-  (** A simplified variant of weakest preconditions for path evaluation.
-      The difference is that path evaluation is completely pure, and
-      postconditions must hold now, not after updating resources.
-      vp ("Value from Path") and vq range over results of evaluating paths.
-
-      Path evaluation was initially more complex; now that we got to this
-      version, I wonder whether we can just use the standard Iris WP, but I am
-      not sure if that would work.
-      *)
-  Fixpoint path_wp p φ: iProp Σ :=
+  (** The definition of total weakest preconditions is very similar to the
+  definition of normal (i.e. partial) weakest precondition, with the exception
+  that there is no later modality. Hence, instead of taking a Banach's fixpoint,
+  we take a least fixpoint. *)
+  Definition path_wp_pre (path_wp : pathO → (vl -d> iPropO Σ) → iProp Σ) p φ : iProp Σ :=
     match p with
-    | pself p l => path_wp p (λ v, ∃ w, ⌜ v @ l ↘ dvl w ⌝ ∧ φ w)
     | pv vp => φ vp
+    | pself p l => ∃ vp q, ⌜ vp @ l ↘ dvl q ⌝ ∧
+        path_wp p (λ v, ⌜ vp = v ⌝) ∗ path_wp q φ
     end%I.
+  Instance: (∀ v, Persistent (φ v)) → (∀ p φ, Persistent (path_wp p φ)) → Persistent (path_wp_pre path_wp p φ).
+  Proof. intros; destruct p; apply _. Qed.
 
-  Global Instance path_wp_ne p : NonExpansive (path_wp p).
+  Lemma path_wp_pre_mono (wp1 wp2 : path → (vl -d> iPropO Σ) → iProp Σ) :
+    ((□ ∀ p Φ, wp1 p Φ -∗ wp2 p Φ) →
+    ∀ p Φ, path_wp_pre wp1 p Φ -∗ path_wp_pre wp2 p Φ)%I.
   Proof.
-    elim: p => [w|p IHp l] n x y Heq /=. done.
-    f_equiv => vp. f_equiv => vq. f_equiv. exact: Heq.
+    iIntros "#H"; iIntros (p1 Φ). rewrite /path_wp_pre /=.
+    destruct (p1) as [v|]; first by iIntros.
+    iDestruct 1 as (vp q Hlook) "[Hp Hq]".
+    iExists vp, q. iFrame (Hlook).
+    iSplitL "Hp"; by iApply "H".
+  Qed.
+
+  (* Uncurry [path_wp_pre] and equip its type with an OFE structure *)
+  Definition path_wp_pre' :
+    (prodO pathO (vl -d> iPropO Σ) → iPropO Σ) →
+    (prodO pathO (vl -d> iPropO Σ) → iPropO Σ) := curry ∘ path_wp_pre ∘ uncurry.
+End path_wp_pre.
+
+Local Instance path_wp_pre_mono' {Σ}: BiMonoPred (@path_wp_pre' Σ).
+Proof.
+  constructor.
+  - iIntros (wp1 wp2) "#H". iIntros ([p Φ]); iRevert (p Φ).
+    iApply path_wp_pre_mono. iIntros "!>" (p Φ). iApply ("H" $! (p,Φ)).
+  - intros wp Hwp n [p1 Φ1] [p2 Φ2] [?%leibniz_equiv Heq]; simplify_eq/=.
+    rewrite /uncurry /path_wp_pre; repeat (apply Heq || f_equiv || done).
+Qed.
+
+Definition path_wp_def {Σ} p φ : iProp Σ := bi_least_fixpoint path_wp_pre' (p, φ).
+Definition path_wp_aux {Σ} : seal (@path_wp_def Σ). by eexists. Qed.
+
+Section path_wp.
+  Context {Σ : gFunctors}.
+  Definition path_wp := (@path_wp_aux Σ).(unseal).
+  Definition path_wp_unseal : path_wp = @path_wp_def Σ := path_wp_aux.(seal_eq).
+
+  Implicit Types (φ Φ : vl -d> iPropO Σ).
+
+  Lemma path_wp_unfold p Φ : path_wp p Φ ⊣⊢ path_wp_pre path_wp p Φ.
+  Proof. by rewrite path_wp_unseal /path_wp_def least_fixpoint_unfold. Qed.
+
+  Lemma path_wp_pv v φ : path_wp (pv v) φ ⊣⊢ φ v.
+  Proof. by rewrite path_wp_unfold. Qed.
+  Lemma path_wp_pself p l φ : path_wp (pself p l) φ ⊣⊢ ∃ vp q, ⌜ vp @ l ↘ dvl q ⌝ ∧
+        path_wp p (λ v, ⌜ vp = v ⌝) ∗ path_wp q φ.
+  Proof. by rewrite path_wp_unfold. Qed.
+
+  (* General induction principle on path_wp. *)
+  Lemma path_wp_ind' Ψ
+    (HΨ : ∀ n p, Proper (pointwise_relation _ (dist n) ==> dist n) (Ψ p)):
+    (□ (∀ p Φ, path_wp_pre (λ p Φ, Ψ p Φ ∧ path_wp p Φ) p Φ -∗ Ψ p Φ) →
+    ∀ p Φ, path_wp p Φ -∗ Ψ p Φ)%I.
+  Proof.
+    iIntros "#IH" (p Φ) "H". rewrite path_wp_unseal.
+    set (Ψ' := curry Ψ : prodO pathO (vl -d> iPropO Σ) → iPropO Σ).
+    have ?: NonExpansive Ψ'.
+    { intros n [p1 Φ1] [p2 Φ2] [?%leibniz_equiv ?]; simplify_eq/=. by apply HΨ. }
+    iApply (least_fixpoint_strong_ind _ Ψ' with "[] H").
+    iIntros "!#" ([? ?]) "H". by iApply "IH".
+  Qed.
+
+  (* Specialized induction principle on path_wp. *)
+  Lemma path_wp_ind Ψ
+    (Hprop : ∀ n p, Proper (pointwise_relation _ (dist n) ==> dist n) (Ψ p)):
+    ((∀ v Φ, □ (Φ v -∗ Ψ (pv v) Φ)) →
+     (∀ p l Φ, □ (path_wp_pre (λ p Φ, Ψ p Φ ∧ path_wp p Φ) (pself p l) Φ -∗ Ψ (pself p l) Φ)) →
+     ∀ p Φ, path_wp p Φ -∗ Ψ p Φ)%I.
+  Proof.
+    iIntros "#Hpv #Hpself" (p Φ) "Hp". iApply (path_wp_ind' with "[] Hp").
+    iIntros "!>" ([|?p l]); iIntros; by [iApply "Hpv"| iApply "Hpself"].
+  Qed.
+
+  Global Instance path_wp_ne p n :
+    Proper (pointwise_relation _ (dist n) ==> dist n) (path_wp p).
+  Proof.
+    intros Φ1 Φ2 HΦ. rewrite !path_wp_unseal. by apply least_fixpoint_ne, pair_ne, HΦ.
+  Qed.
+  Global Instance path_wp_ne' p : NonExpansive (path_wp p).
+  Proof. solve_proper. Qed.
+
+  Global Instance path_wp_proper p :
+    Proper (pointwise_relation _ (≡) ==> (≡)) (path_wp p).
+  Proof.
+    by intros Φ Φ' ?; apply equiv_dist=>n; apply path_wp_ne=>v; apply equiv_dist.
   Qed.
 
   Global Instance path_wp_persistent φ p:
     (∀ v, Persistent (φ v)) → Persistent (path_wp p φ).
-  Proof. elim: p φ => *; apply _. Qed.
+  Proof.
+    rewrite /Persistent => Hφ.
+    (* Make Hφ internal, or the required non-expansiveness will be false. *)
+    iAssert (∀ v, φ v -∗ <pers> φ v)%I as "Hv". by iIntros; iApply Hφ.
+    clear Hφ; iIntros "H"; iRevert (p φ) "H Hv".
+
+    iApply path_wp_ind; first solve_proper; iIntros;
+      rewrite /path_wp_pre path_wp_unfold /=; iModIntro.
+    by iIntros "Hv HP"; iApply "HP".
+    iDestruct 1 as (vp q Hlook) "[[IHeq _] [IHpw _]]"; iIntros "HP".
+    iApply persistently_exist; iExists vp.
+    iApply persistently_exist; iExists q.
+    iApply persistently_and; iSplit; first by eauto.
+    iApply persistently_sep; iSplit;
+      [iApply "IHeq"; eauto | iApply ("IHpw" with "HP")].
+  Qed.
 
   Global Instance Proper_pwp: Proper ((=) ==> pointwise_relation _ (≡) ==> (≡)) path_wp.
   Proof.
     (* The induction works best in this shape, but this instance is best kept local. *)
     have Proper_pwp_2: ∀ p, Proper (pointwise_relation _ (≡) ==> (≡)) (path_wp p).
-    elim; solve_proper.
+    by apply _.
     solve_proper.
   Qed.
 
   Lemma path_wp_pureable p Pv:
     path_wp p (λ v, ⌜Pv v⌝) ⊣⊢ ⌜path_wp_pure p Pv⌝.
   Proof.
-    elim: p Pv => /= [//|p IHp l] Pv.
-    by rewrite -{}IHp; f_equiv => v; iIntros "!% /=".
+    iSplit.
+    - move HE: (λ v : vl, ⌜Pv v⌝)%I => φ.
+      (* Internalize HE to ensure properness. *)
+      iAssert ((φ : vl -d> iPropO Σ) ≡ (λ v : vl, ⌜Pv v⌝))%I as "HE".
+      by simplify_eq.
+      clear HE.
+      iIntros "H"; iRevert (Pv) "HE"; iRevert (p φ) "H".
+      iApply path_wp_ind; first solve_proper; iIntros; iModIntro.
+      + iIntros "Hv" (Pv) "Heq"; rewrite bi.discrete_fun_equivI /=.
+        iRewrite ("Heq" $! v) in "Hv". iDestruct "Hv" as %Hv. auto.
+      + iDestruct 1 as (vp q Hlook) "[[IHp _] [IHq _]]"; iIntros (Pv) "Heq".
+        iDestruct ("IHq" with "Heq") as %Hq.
+        iDestruct ("IHp" with "[//]") as %Hp.
+        eauto.
+    - iIntros (Hp); iInduction Hp as [] "IH"; iEval (rewrite path_wp_unfold /=); eauto.
   Qed.
 
   Lemma path_wp_wand φ1 φ2 p:
@@ -202,11 +324,13 @@ Section path_wp.
     (∀ v, φ1 v -∗ φ2 v) -∗
     path_wp p φ2.
   Proof.
-    elim: p φ1 φ2 => /= [v|p IHp l] ??; iIntros "H1 Hwand";
-      first by iApply "Hwand".
-    iApply (IHp with "H1").
-    iIntros (v); iDestruct 1 as (vq Hl) "?".
-    iExists vq; iFrame (Hl). by iApply "Hwand".
+    iIntros "H1". iRevert (φ2). iRevert (p φ1) "H1".
+    iApply path_wp_ind; first solve_proper; rewrite /path_wp_pre /=; iIntros; iModIntro.
+    by iIntros "H1" (Φ2) "Hwand"; rewrite path_wp_unfold/=; iApply "Hwand".
+    iDestruct 1 as (vp q Hlook) "[[IHp Hp] IHq]"; iIntros (Φ2) "Hwand".
+    iEval (rewrite path_wp_unfold /=).
+    iExists vp, q; iFrame (Hlook) "Hp".
+    iApply ("IHq" with "Hwand").
   Qed.
 
   Global Instance path_wp_pureableI p φ Pv :
@@ -238,25 +362,64 @@ Section path_wp.
   Lemma path_wp_eq p φ :
     path_wp p φ ⊣⊢ ∃ v, ⌜ path_wp_pure p (eq v) ⌝ ∧ φ v.
   Proof.
-    elim: p φ => [ v | p IHp l ] φ /=; iSplit; iIntros "H".
-    - auto.
-    - by iDestruct "H" as (w <-) "H".
-    - rewrite IHp.
-      iDestruct "H" as (v Hp w Hl) "Hw".
-      iExists w; iSplit; last by [].
-      iIntros "!%". apply: path_wp_pure_wand; naive_solver.
-    - setoid_rewrite IHp; setoid_rewrite path_wp_pure_eq.
-      iDestruct "H" as (w [v Hp]) "Hw".
-      iExists v; iSplit; naive_solver eauto.
+    iSplit.
+    - iRevert (p φ); iApply path_wp_ind; first solve_proper;
+      rewrite /path_wp_pre /=; iIntros; iModIntro.
+      + by iIntros "H"; iExists v; eauto.
+      + iDestruct 1 as (vp q Hlook) "[[IHp _] [IHq _]]".
+        iDestruct "IHp" as %(? & Hp & <-).
+        iDestruct "IHq" as (vq Hq) "H".
+        iExists vq; eauto.
+    - iDestruct 1 as (v Hwp) "H".
+      move: Hwp; move HE: (eq v) => φ' Hwp.
+      iInduction Hwp as [|] "IH"; simplify_eq/=;
+        iEval (rewrite path_wp_unfold /=); first done.
+      iExists _, _; repeat iSplit => //.
+      by iApply "IH1".
+  Qed.
+
+  Notation PersistentP Φ := (∀ v, Persistent (Φ v)).
+
+  Lemma path_wp_and p Φ1 Φ2 `{PersistentP Φ1} `{PersistentP Φ2}:
+    path_wp p Φ1 ∧ path_wp p Φ2 ⊣⊢
+    path_wp p (λ v, Φ1 v ∧ Φ2 v).
+  Proof.
+    rewrite !path_wp_eq; iSplit.
+    - iIntros "[H1 H2]".
+      iDestruct "H1" as (v1 Hv1) "H1"; iDestruct "H2" as (v2 Hv2) "H2".
+      rewrite -(path_wp_pure_det Hv1 Hv2); iExists v1; eauto.
+    - iDestruct 1 as (v Hv) "[H1 H2]"; eauto 6.
+  Qed.
+
+  Lemma path_wp_or p Φ1 Φ2 `{PersistentP Φ1} `{PersistentP Φ2}:
+    path_wp p Φ1 ∨ path_wp p Φ2 ⊣⊢
+    path_wp p (λ v, Φ1 v ∨ Φ2 v).
+  Proof.
+    rewrite !path_wp_eq; iSplit.
+    - iIntros "[H|H]"; iDestruct "H" as (v Hv) "H"; eauto.
+    - iDestruct 1 as (v Hv) "[H|H]"; eauto.
   Qed.
 
   Lemma path_wp_later_swap p φ:
     path_wp p (λ v, ▷ φ v) ⊢ ▷ path_wp p (λ v, φ v).
   Proof.
-    elim: p φ => [v // | p IHp l /=] φ.
-    rewrite -IHp.
-    iIntros "H"; iApply (path_wp_wand with "H").
-    by iIntros (v) "H !>".
+    iIntros "HP".
+    move HE: (λ v, ▷ φ v)%I => Φ.
+    iAssert ((Φ : vl -d> iPropO Σ) ≡ (λ v, ▷ φ v))%I as "HE".
+    by simplify_eq.
+    clear HE.
+    iRevert (p Φ) "HP HE".
+
+    iApply path_wp_ind; first solve_proper;
+      rewrite /path_wp_pre /=; iIntros; iModIntro.
+    - iIntros "HP Heq"; rewrite bi.discrete_fun_equivI path_wp_unfold /=.
+      by iRewrite ("Heq" $! v) in "HP".
+    - iDestruct 1 as (vp q Hlook) "[[IHp Hp] [IHq _]]".
+      iIntros "Heq".
+      iEval rewrite path_wp_unfold; rewrite !bi.discrete_fun_equivI /=.
+      iExists vp, q; repeat iSplit => //.
+      by iApply "IHq".
+      (* Why no more [path_wp_wand]? *)
   Qed.
 
   Lemma path_wp_laterN_swap p φ i:
