theories/Dot/misc_unused/misc_dead.v
@@ -90,9 +90,9 @@ Proof.
   apply _.
 Abort. *)
 
-Lemma dms_lookup_subst l ds w ρ :
-  dms_lookup l (selfSubst ds) = Some (dvl w) →
-  dms_lookup l (selfSubst ds.|[up ρ]) = Some (dvl w.[ρ]).
+Lemma dms_lookup_subst l ds p ρ :
+  dms_lookup l (selfSubst ds) = Some (dvl p) →
+  dms_lookup l (selfSubst ds.|[up ρ]) = Some (dvl p.|[ρ]).
 Proof.
   rewrite /selfSubst (subst_swap _ _ (vobj ds)).
   move: (vobj ds) => v0.
@@ -107,7 +107,7 @@ Proof.
   - have <-: t1.|[up ρ].|[v2.[ρ]/] = t1.|[v2/].|[ρ].
     by rewrite subst_swap.
     by constructor.
-  - intros [ds [-> Hl]].
+  - intros [ds [-> Hl]]; rewrite path2tm_subst.
     constructor.
     eexists ds.|[up ρ]; split => //.
     exact: dms_lookup_subst.
